towards support for Delete
the main lock-based pickup/delete logic is proven (MailboxImpl.v)

need to prove MailServerLockAbsImpl.v, and propagate Delete/Lock/Unlock
down the stack.

src/Mail2/MailboxAPI.v
@@ -1,69 +1,140 @@
 Require Import POCS.
 Require Import String.
 Require Import MailServerAPI.
+Require Import MailServerLockAbsAPI.
 
 
 Module MailboxAPI <: Layer.
 
   Import MailServerAPI.
+  Import MailServerLockAbsAPI.
 
   Inductive xopT : Type -> Type :=
   | Deliver : forall (m : string), xopT unit
   | List : xopT (list (nat*nat))
   | Read : forall (fn : nat*nat), xopT (option string)
+  | Delete : forall (fn : nat*nat), xopT unit
+  | Lock : xopT unit
+  | Unlock : xopT unit
   | GetRequest : xopT request
   | Respond : forall (T : Type) (v : T), xopT unit
   .
 
   Definition opT := xopT.
-  Definition State := dir_contents.
+  Definition State := MailServerLockAbsAPI.State.
   Definition initP (s : State) := True.
 
   Inductive xstep : forall T, opT T -> nat -> State -> T -> State -> list event -> Prop :=
-  | StepDeliver : forall m mbox tid fn,
+  | StepDeliver : forall m mbox tid fn lock,
     ~ FMap.In fn mbox ->
     xstep (Deliver m) tid
-      mbox
+      (mk_state mbox lock)
       tt
-      (FMap.add fn m mbox)
+      (mk_state (FMap.add fn m mbox) lock)
       nil
-  | StepList : forall mbox tid r,
+  | StepList : forall mbox tid r lock,
     FMap.is_permutation_key r mbox ->
     xstep List tid
-      mbox
+      (mk_state mbox lock)
       r
-      mbox
+      (mk_state mbox lock)
       nil
 
-  | StepReadOK : forall fn mbox tid m,
+  | StepReadOK : forall fn mbox tid m lock,
     FMap.MapsTo fn m mbox ->
     xstep (Read fn) tid
-      mbox
+      (mk_state mbox lock)
       (Some m)
-      mbox
+      (mk_state mbox lock)
       nil
-  | StepReadNone : forall fn mbox tid,
+  | StepReadNone : forall fn mbox tid lock,
     ~ FMap.In fn mbox ->
     xstep (Read fn) tid
-      mbox
+      (mk_state mbox lock)
       None
-      mbox
+      (mk_state mbox lock)
       nil
 
-  | StepGetRequest : forall mbox tid r,
-    xstep GetRequest tid
-      mbox
-      r
-      mbox
-      (Event r :: nil)
-  | StepRespond : forall mbox tid T (v : T),
-    xstep (Respond v) tid
-      mbox
+  | StepDelete : forall fn mbox tid lock,
+    xstep (Delete fn) tid
+      (mk_state mbox lock)
       tt
-      mbox
+      (mk_state (FMap.remove fn mbox) lock)
+      nil
+
+  | StepLock : forall mbox tid,
+    xstep Lock tid
+      (mk_state mbox None)
+      tt
+      (mk_state mbox (Some tid))
+      nil
+  | StepUnlock : forall mbox tid lock,
+    xstep Unlock tid
+      (mk_state mbox lock)
+      tt
+      (mk_state mbox None)
+      nil
+
+  | StepGetRequest : forall st tid r,
+    xstep GetRequest tid
+      st
+      r
+      st
+      (Event r :: nil)
+  | StepRespond : forall st tid T (v : T),
+    xstep (Respond v) tid
+      st
+      tt
+      st
       (Event v :: nil)
   .
 
   Definition step := xstep.
 
 End MailboxAPI.
+
+
+Module MailboxRestrictedAPI <: Layer.
+
+  Import MailboxAPI.
+  Import MailServerLockAbsAPI.
+
+  Definition opT := MailboxAPI.opT.
+  Definition State := MailboxAPI.State.
+  Definition initP := MailboxAPI.initP.
+
+  Inductive step_allow : forall T, opT T -> nat -> State -> Prop :=
+  | AllowDeliver : forall m tid s,
+    step_allow (Deliver m) tid s
+  | AllowList : forall tid s,
+    step_allow List tid s
+  | AllowRead : forall fn tid s,
+    locked s = Some tid ->
+    step_allow (Read fn) tid s
+  | AllowDelete : forall fn tid s,
+    locked s = Some tid ->
+    step_allow (Delete fn) tid s
+  | AllowLock : forall tid s,
+    step_allow Lock tid s
+  | AllowUnlock : forall tid s,
+    locked s = Some tid ->
+    step_allow Unlock tid s
+  | AllowGetRequest : forall tid s,
+    step_allow GetRequest tid s
+  | AllowRespond : forall `(r : T) tid s,
+    step_allow (Respond r) tid s
+  .
+
+  Definition step :=
+    restricted_step MailboxAPI.step step_allow.
+
+End MailboxRestrictedAPI.
+
+
+Module MailboxLockingRule <: ProcRule MailboxAPI.
+
+  Definition follows_protocol (ts : @threads_state MailboxAPI.opT) :=
+    forall s,
+      follows_protocol_s MailboxAPI.step MailboxRestrictedAPI.step_allow ts s.
+
+End MailboxLockingRule.
