src/Mail2/MailboxImpl.v
@@ -2,14 +2,17 @@ Require Import POCS.
 Require Import String.
 Require Import MailboxAPI.
 Require Import MailServerAPI.
+Require Import MailServerLockAbsAPI.
 Require Import FMapFacts.
 
 
-Module AtomicReader <: LayerImpl MailboxAPI MailServerAPI.
+Module AtomicReaderRestricted <: LayerImplFollowsRule MailboxRestrictedAPI MailServerLockAbsAPI MailboxLockingRule.
 
   Fixpoint read_list (l : list (nat*nat)) (r : list ((nat*nat) * string)) :=
     match l with
-    | nil => Ret r
+    | nil =>
+      _ <- Op MailboxAPI.Unlock;
+      Ret r
     | fn :: l' =>
       m <- Op (MailboxAPI.Read fn);
       match m with
@@ -19,13 +22,21 @@ Module AtomicReader <: LayerImpl MailboxAPI MailServerAPI.
     end.
 
   Definition pickup_core :=
+    _ <- Op MailboxAPI.Lock;
     l <- Op MailboxAPI.List;
     read_list l nil.
 
-  Definition compile_op T (op : MailServerAPI.opT T) : proc _ T :=
+  Definition delete_core fn :=
+    _ <- Op MailboxAPI.Lock;
+    _ <- Op (MailboxAPI.Delete fn);
+    _ <- Op MailboxAPI.Unlock;
+    Ret tt.
+
+  Definition compile_op T (op : MailServerLockAbsAPI.opT T) : proc _ T :=
     match op with
     | MailServerAPI.Deliver m => Op (MailboxAPI.Deliver m)
     | MailServerAPI.Pickup => pickup_core
+    | MailServerAPI.Delete fn => delete_core fn
     | MailServerAPI.GetRequest => Op (MailboxAPI.GetRequest)
     | MailServerAPI.Respond r => Op (MailboxAPI.Respond r)
     end.
@@ -34,13 +45,19 @@ Module AtomicReader <: LayerImpl MailboxAPI MailServerAPI.
     match goal with
     | H : MailboxAPI.step _ _ _ _ _ _ |- _ =>
       inversion H; clear H; subst; repeat sigT_eq
-    | H : MailServerAPI.step _ _ _ _ _ _ |- _ =>
+    | H : MailboxRestrictedAPI.step _ _ _ _ _ _ |- _ =>
+      inversion H; clear H; subst; repeat sigT_eq
+    | H : MailboxRestrictedAPI.step_allow _ _ _ |- _ =>
+      inversion H; clear H; subst; repeat sigT_eq
+    | H : MailServerLockAbsAPI.step _ _ _ _ _ _ |- _ =>
       inversion H; clear H; subst; repeat sigT_eq
     end; intuition idtac.
 
   Hint Extern 1 (MailboxAPI.step _ _ _ _ _ _) => econstructor.
-  Hint Extern 1 (MailServerAPI.step _ _ _ _ _ _) => econstructor.
+  Hint Extern 1 (MailServerLockAbsAPI.step _ _ _ _ _ _) => econstructor.
+  Hint Extern 1 (MailboxRestrictedAPI.step _ _ _ _ _ _) => econstructor.
   Hint Constructors MailboxAPI.xstep.
+  Hint Constructors MailboxRestrictedAPI.step_allow.
 
   Hint Resolve FMap.mapsto_in.
   Hint Resolve FMap.mapsto_add_ne'.
@@ -48,48 +65,88 @@ Module AtomicReader <: LayerImpl MailboxAPI MailServerAPI.
   Hint Resolve FMap.add_incr.
   Hint Resolve FMap.add_mapsto.
   Hint Resolve FMap.in_add_ne.
+  Hint Resolve FMap.remove_not_in.
+  Hint Resolve FMap.mapsto_remove_ne.
 
   Lemma read_left_mover : forall fn,
     left_mover_pred
-      MailboxAPI.step
+      MailboxRestrictedAPI.step
       (MailboxAPI.Read fn)
-      (fun tid s => FMap.In fn s).
+      (fun tid s => FMap.In fn (MailServerLockAbsAPI.maildir s)).
   Proof.
     split.
     - unfold enabled_stable, enabled_in; intros; repeat deex.
-      unfold MailboxAPI.step.
+      unfold MailboxRestrictedAPI.step, MailboxAPI.step, restricted_step.
       destruct rM; try congruence.
-      + repeat step_inv; eauto; try congruence.
+      + repeat step_inv; eauto 10; simpl in *; try congruence.
         destruct (fn == fn0); subst; eauto 10.
-      + repeat step_inv; eauto; try congruence.
+      + repeat step_inv; eauto 7; simpl in *; try congruence.
         destruct (fn0 == fn); subst; eauto 10.
-    - intros; repeat step_inv; eauto; repeat deex.
+    - intros; repeat step_inv; eauto 10; repeat deex; simpl in *; try congruence.
       + destruct (fn0 == fn); subst; try congruence.
         eauto 10.
       + destruct (fn0 == fn); subst; try congruence.
-        eauto 10.
+        eauto 15.
+  Qed.
+
+  Lemma unlock_left_mover :
+    left_mover
+      MailboxRestrictedAPI.step
+      MailboxAPI.Unlock.
+  Proof.
+    split.
+    - unfold enabled_stable, enabled_in; intros; repeat deex.
+      unfold MailboxRestrictedAPI.step, MailboxAPI.step, restricted_step.
+      repeat step_inv; eauto 7; simpl in *; try congruence.
+    - intros; repeat step_inv; eauto 10; repeat deex; simpl in *; try congruence.
+  Qed.
+
+  Lemma lock_right_mover :
+    right_mover
+      MailboxRestrictedAPI.step
+      MailboxAPI.Lock.
+  Proof.
+    unfold right_mover; intros.
+    repeat step_inv; simpl in *; try congruence; eauto 10.
   Qed.
 
   Hint Resolve read_left_mover.
+  Hint Resolve unlock_left_mover.
+  Hint Resolve lock_right_mover.
 
-  Lemma mailbox_fn_monotonic :
-    forall s s' tid fn,
-      exec_others MailboxAPI.step tid s s' ->
-      FMap.In fn s ->
-      FMap.In fn s'.
+  Hint Resolve FMap.add_incr.
+
+  Lemma lock_monotonic :
+    forall s s' tid,
+      exec_others MailboxRestrictedAPI.step tid s s' ->
+      MailServerLockAbsAPI.locked s = Some tid ->
+        MailServerLockAbsAPI.locked s' = Some tid.
   Proof.
     induction 1; eauto; intros.
     repeat deex.
     eapply IHclos_refl_trans_1n; clear IHclos_refl_trans_1n.
-    clear H0.
-    step_inv.
-    eapply FMap.add_incr; eauto.
+    repeat step_inv; simpl in *; try congruence.
+  Qed.
+
+  Lemma mailbox_fn_monotonic :
+    forall s s' tid fn,
+      exec_others MailboxRestrictedAPI.step tid s s' ->
+      MailServerLockAbsAPI.locked s = Some tid ->
+      FMap.In fn (MailServerLockAbsAPI.maildir s) ->
+        MailServerLockAbsAPI.locked s' = Some tid /\
+        FMap.In fn (MailServerLockAbsAPI.maildir s').
+  Proof.
+    induction 1; eauto; intros.
+    repeat deex.
+    eapply IHclos_refl_trans_1n; clear IHclos_refl_trans_1n.
+    - repeat step_inv; simpl in *; try congruence.
+    - repeat step_inv; simpl in *; try congruence; eauto.
   Qed.
 
   Hint Resolve FMap.is_permutation_in.
 
   Theorem pickup_atomic : forall `(rx : _ -> proc _ T),
-    trace_incl MailboxAPI.step
+    trace_incl MailboxRestrictedAPI.step
       (Bind (compile_op MailServerAPI.Pickup) rx)
       (Bind (atomize compile_op MailServerAPI.Pickup) rx).
   Proof.
@@ -97,80 +154,139 @@ Module AtomicReader <: LayerImpl MailboxAPI MailServerAPI.
     eapply trace_incl_atomize_ysa.
     simpl.
     unfold pickup_core, ysa_movers.
-    eapply RightMoversDone.
-    eapply OneNonMover.
 
-    intros.
+    eapply RightMoversOne; eauto; intros.
+    destruct r.
+
+    eapply RightMoversDone.
+
+    eapply OneNonMover; intros.
+
     eapply left_movers_impl with
-      (P1 := fun tid s => Forall (fun fn => FMap.In fn s) r).
+      (P1 := fun tid s =>
+        MailServerLockAbsAPI.locked s = Some tid /\
+        Forall (fun fn => FMap.In fn (MailServerLockAbsAPI.maildir s)) r).
 
     {
       generalize (@nil ((nat*nat) * string)).
-      induction r; simpl; eauto.
-      constructor; eauto.
+      induction r; simpl; eauto; intros.
+
+      {
+        constructor; eauto.
+        intuition eauto.
+        destruct s; unfold enabled_in.
+        eauto 10.
+      }
+
+      constructor; intuition idtac.
 
       - eapply left_mover_pred_impl; eauto.
-        intros.
-        inversion H; clear H; subst.
+        intuition idtac.
+        inversion H1; clear H1; subst.
         eauto.
 
-      - intros.
-        inversion H; clear H; subst.
-        eapply FMap.in_mapsto_exists in H2; deex.
+      - inversion H1; clear H1; subst.
+        eapply FMap.in_mapsto_exists in H3; deex.
+        destruct s; simpl in *.
         do 2 eexists; econstructor; eauto.
 
-      - intros.
-        destruct r0; subst; try congruence.
-        ++ eapply left_movers_impl; eauto.
-           intros; repeat deex.
-           inversion H; clear H; subst.
+      - destruct r0; subst; try congruence.
+       ++ eapply left_movers_impl; eauto.
+          intros; repeat deex.
+          inversion H2; clear H2; subst.
 
-           eapply exec_any_op in H0; repeat deex.
-           step_inv.
+          eapply exec_any_op in H0; repeat deex.
+          eapply mailbox_fn_monotonic in H0 as H0'; [ | intuition eauto.. ].
+          repeat step_inv.
 
-           eapply Forall_impl; eauto; intros; simpl in *.
-           eapply mailbox_fn_monotonic; eauto.
-           eapply mailbox_fn_monotonic; eauto.
-           inversion H9.
-       ++  eapply left_movers_impl; eauto.
-           intros; repeat deex.
-           inversion H; clear H; subst.
+          eapply mailbox_fn_monotonic in H1; intuition eauto.
 
-           eapply exec_any_op in H0; repeat deex.
-           step_inv.
-           inversion H9.
+          eapply Forall_impl; eauto; intros; simpl in *.
+          eapply mailbox_fn_monotonic; eauto.
+          eapply mailbox_fn_monotonic; eauto.
 
-           eapply Forall_impl; eauto; intros; simpl in *.
-           eapply mailbox_fn_monotonic; eauto.
-           eapply mailbox_fn_monotonic; eauto.
+      ++  eapply left_movers_impl; eauto.
+          intros; repeat deex.
+          inversion H2; clear H2; subst.
+
+          eapply exec_any_op in H0; repeat deex.
+          eapply mailbox_fn_monotonic in H0 as H0'; [ | intuition eauto.. ].
+          repeat step_inv.
+
+          eapply mailbox_fn_monotonic in H1; intuition eauto.
+
+          eapply Forall_impl; eauto; intros; simpl in *.
+          eapply mailbox_fn_monotonic; eauto.
+          eapply mailbox_fn_monotonic; eauto.
     }
 
     intros; repeat deex.
+    eapply exec_any_op in H2; repeat deex.
     eapply exec_any_op in H0; repeat deex.
-    step_inv.
-    eapply Forall_in'; intros.
+    repeat step_inv.
 
-    eapply mailbox_fn_monotonic; eauto.
+    eapply lock_monotonic in H3; simpl in *; subst; [ | congruence ].
+    eapply lock_monotonic in H0; simpl in *; subst; [ | congruence ].
+    eapply lock_monotonic in H1; simpl in *; subst; [ | congruence ].
+    eauto.
+
+    eapply lock_monotonic in H3; simpl in *; subst; [ | congruence ].
+    eapply lock_monotonic in H0; simpl in *; subst; [ | congruence ].
+
+    eapply Forall_in'; intros.
+    eapply mailbox_fn_monotonic in H1; intuition eauto.
+  Qed.
+
+  Theorem delete_atomic : forall `(rx : _ -> proc _ T) fn,
+    trace_incl MailboxRestrictedAPI.step
+      (Bind (compile_op (MailServerAPI.Delete fn)) rx)
+      (Bind (atomize compile_op (MailServerAPI.Delete fn)) rx).
+  Proof.
+    intros.
+    eapply trace_incl_atomize_ysa.
+    simpl.
+    unfold delete_core, ysa_movers.
+
+    eapply RightMoversOne; eauto; intros.
+    eapply RightMoversDone.
+    eapply OneNonMover; intros.
+    eapply LeftMoversOne; eauto.
+
+    intros.
+    repeat deex.
+
+    eapply exec_any_op in H2; repeat deex.
+    eapply exec_any_op in H0; repeat deex.
+    repeat step_inv.
+
+    eapply lock_monotonic in H3; simpl in *; subst; [ | congruence ].
+    eapply lock_monotonic in H1; simpl in *; subst; [ | congruence ].
+
+    destruct s.
+    do 3 eexists. eauto.
   Qed.
 
   Lemma read_list_exec : forall l r s s' evs v tid,
-    List.Forall (fun fn => FMap.In fn s) l ->
-    Forall (fun '(fn, m) => FMap.MapsTo fn m s) r ->
-    atomic_exec MailboxAPI.step
+    List.Forall (fun fn => FMap.In fn (MailServerLockAbsAPI.maildir s)) l ->
+    Forall (fun '(fn, m) => FMap.MapsTo fn m (MailServerLockAbsAPI.maildir s)) r ->
+    atomic_exec MailboxRestrictedAPI.step
       (read_list l r) tid
       s v s' evs ->
-    s' = s /\ evs = nil /\
-    Forall (fun '(fn, m) => FMap.MapsTo fn m s) v /\
+    MailServerLockAbsAPI.maildir s' = MailServerLockAbsAPI.maildir s /\
+    MailServerLockAbsAPI.locked s' = None /\
+    evs = nil /\
+    Forall (fun '(fn, m) => FMap.MapsTo fn m (MailServerLockAbsAPI.maildir s)) v /\
     map fst r ++ l = map fst v.
   Proof.
     induction l; intros.
-    - atomic_exec_inv.
+    - repeat atomic_exec_inv.
+      repeat step_inv.
       rewrite app_nil_r.
       eauto.
     - atomic_exec_inv.
+      inversion H11; clear H11; subst; repeat sigT_eq.
       destruct v1; subst; try congruence.
-      + inversion H11; clear H11; subst; repeat sigT_eq.
-        edestruct IHl; [ | | eauto | ]; step_inv.
+      + edestruct IHl; [ | | eauto | ]; repeat step_inv.
         all: try inversion H7; subst; try congruence.
        -- inversion H; subst; eauto.
        -- eapply Forall_forall; intros.
@@ -179,42 +295,44 @@ Module AtomicReader <: LayerImpl MailboxAPI MailServerAPI.
           * repeat match goal with
             | H : In _ _ |- _ => inversion H; clear H; subst
             end; eauto.
+            inversion H8; subst; eauto.
        -- rewrite map_app in *.
           rewrite <- app_assoc in *.
           simpl in *.
           eauto.
       + exfalso.
-        inversion H11; clear H11; subst; repeat sigT_eq.
         eapply Forall_inv in H.
-        step_inv.
+        repeat step_inv.
         congruence.
   Qed.
 
   Theorem my_compile_correct :
-    compile_correct compile_op MailboxAPI.step MailServerAPI.step.
+    compile_correct compile_op MailboxRestrictedAPI.step MailServerLockAbsAPI.step.
   Proof.
     unfold compile_correct; intros.
     destruct op.
 
     + repeat atomic_exec_inv.
-      simpl; intuition eauto.
-      repeat step_inv; eauto.
+      repeat step_inv; eauto 10.
 
     + atomic_exec_inv.
-      eapply read_list_exec in H10.
+      atomic_exec_inv.
+      eapply read_list_exec in H11.
       {
         simpl in *.
-        atomic_exec_inv.
-        step_inv; subst; eauto.
+        repeat atomic_exec_inv.
+        repeat step_inv; subst; eauto.
+        simpl in *; subst.
+        destruct s'; simpl in *; subst.
         econstructor.
 
         eapply FMap.is_permutation_key_to_kv; eauto.
       }
 
       {
-        clear H10.
-        atomic_exec_inv.
-        step_inv.
+        clear H11.
+        repeat atomic_exec_inv.
+        repeat step_inv.
 
         eapply Forall_forall; intros.
         eapply FMap.is_permutation_in; eauto.
@@ -223,21 +341,27 @@ Module AtomicReader <: LayerImpl MailboxAPI MailServerAPI.
       constructor.
 
     + repeat atomic_exec_inv.
-      simpl; intuition eauto.
       repeat step_inv; eauto.
 
     + repeat atomic_exec_inv.
-      simpl; intuition eauto.
-      repeat step_inv; eauto.
+      repeat step_inv.
+      destruct s'; eauto.
+
+    + repeat atomic_exec_inv.
+      repeat step_inv.
+      destruct s'; eauto.
   Qed.
 
   Theorem my_atomize_correct :
-    atomize_correct compile_op MailboxAPI.step.
+    atomize_correct compile_op MailboxRestrictedAPI.step.
   Proof.
     unfold atomize_correct; intros.
     destruct op; try trace_incl_simple.
 
     rewrite pickup_atomic.
+    eapply trace_incl_bind_a; eauto.
+
+    rewrite delete_atomic.
     eapply trace_incl_bind_a; eauto.
   Qed.
 
@@ -247,13 +371,13 @@ Module AtomicReader <: LayerImpl MailboxAPI MailServerAPI.
   Theorem all_traces_match :
     forall ts1 ts2,
       proc_match (Compile.compile_ok compile_op) ts1 ts2 ->
-      traces_match_ts MailboxAPI.step MailServerAPI.step ts1 ts2.
+      traces_match_ts MailboxRestrictedAPI.step MailServerLockAbsAPI.step ts1 ts2.
   Proof.
     intros.
     eapply Compile.compile_traces_match_ts; eauto.
   Qed.
 
-  Definition absR (s1 : MailboxAPI.State) (s2 : MailServerAPI.State) :=
+  Definition absR (s1 : MailboxRestrictedAPI.State) (s2 : MailServerLockAbsAPI.State) :=
     s1 = s2.
 
   Definition compile_ts := Compile.compile_ts compile_op.
@@ -281,7 +405,7 @@ Module AtomicReader <: LayerImpl MailboxAPI MailServerAPI.
   Theorem compile_traces_match :
     forall ts2,
       no_atomics_ts ts2 ->
-      traces_match_abs absR MailboxAPI.initP MailboxAPI.step MailServerAPI.step (compile_ts ts2) ts2.
+      traces_match_abs absR MailboxRestrictedAPI.initP MailboxRestrictedAPI.step MailServerLockAbsAPI.step (compile_ts ts2) ts2.
   Proof.
     unfold traces_match_abs; intros.
     rewrite H2 in *; clear H2.
@@ -291,11 +415,189 @@ Module AtomicReader <: LayerImpl MailboxAPI MailServerAPI.
 
   Theorem absInitP :
     forall s1 s2,
-      MailboxAPI.initP s1 ->
+      MailboxRestrictedAPI.initP s1 ->
       absR s1 s2 ->
-      MailServerAPI.initP s2.
+      MailServerLockAbsAPI.initP s2.
   Proof.
     eauto.
   Qed.
 
-End AtomicReader.
+
+  Lemma delete_follows_protocol : forall tid s fn,
+    follows_protocol_proc
+      MailboxAPI.step
+      MailboxRestrictedAPI.step_allow
+      tid s (delete_core fn).
+  Proof.
+    intros.
+    constructor; intros.
+      constructor; intros. eauto.
+
+    eapply exec_any_op in H; repeat deex.
+      unfold restricted_step in *; intuition idtac.
+      repeat step_inv.
+
+    constructor; intros.
+      constructor; intros. eauto.
+
+    eapply exec_any_op in H0; repeat deex.
+      eapply lock_monotonic in H0; try reflexivity.
+      unfold restricted_step in *; intuition idtac.
+      repeat step_inv.
+      simpl in *; subst.
+
+    constructor; intros.
+      constructor; intros. eauto.
+
+    constructor; intros.
+  Qed.
+
+  Lemma pickup_follows_protocol : forall tid s,
+    follows_protocol_proc
+      MailboxAPI.step
+      MailboxRestrictedAPI.step_allow
+      tid s (pickup_core).
+  Proof.
+    intros.
+    constructor; intros.
+      constructor; intros. eauto.
+
+    eapply exec_any_op in H; repeat deex.
+      unfold restricted_step in *; intuition idtac.
+      repeat step_inv.
+
+    constructor; intros.
+      constructor; intros. eauto.
+
+    eapply exec_any_op in H0; repeat deex.
+      eapply lock_monotonic in H0; try reflexivity.
+      unfold restricted_step in *; intuition idtac.
+      repeat step_inv.
+      simpl in *; subst.
+
+    clear.
+    generalize dependent mbox0.
+    generalize (@nil ((nat*nat) * string)).
+    induction r; simpl; intros.
+
+    - constructor; intros.
+        constructor; intros. eauto.
+
+      constructor; intros.
+
+    - constructor; intros.
+        constructor; intros. eauto.
+
+      eapply exec_any_op in H; repeat deex.
+        eapply lock_monotonic in H; try reflexivity.
+        unfold restricted_step in *; intuition idtac.
+        repeat step_inv; simpl in *; subst; eauto.
+  Qed.
+
+  Hint Resolve delete_follows_protocol.
+  Hint Resolve pickup_follows_protocol.
+
+
+  Theorem compile_ts_follows_protocol :
+    forall ts,
+      no_atomics_ts ts ->
+      MailboxLockingRule.follows_protocol (compile_ts ts).
+  Proof.
+    unfold compile_ts.
+    unfold MailboxLockingRule.follows_protocol.
+    unfold follows_protocol_s.
+    intros.
+    eapply compile_ts_follows_protocol_proc; try eassumption.
+    intros.
+
+    destruct op; simpl; eauto.
+  Qed.
+
+End AtomicReaderRestricted.
+
+
+Module AtomicReaderRestricted' <: LayerImplRequiresRule MailboxAPI MailboxRestrictedAPI MailboxLockingRule.
+
+  Import MailboxLockingRule.
+
+  Definition absR (s1 : MailboxAPI.State) (s2 : MailboxRestrictedAPI.State) :=
+    s1 = s2.
+
+  Ltac step_inv :=
+    match goal with
+    | H : MailboxAPI.step _ _ _ _ _ _ |- _ =>
+      inversion H; clear H; subst; repeat sigT_eq
+    | H : MailboxRestrictedAPI.step_allow _ _ _ |- _ =>
+      inversion H; clear H; subst; repeat sigT_eq
+    | H : MailboxRestrictedAPI.step _ _ _ _ _ _ |- _ =>
+      destruct H; intuition idtac
+    end.
+
+  Theorem allowed_stable :
+    forall `(op : MailboxAPI.opT T) `(op' : MailboxAPI.opT T') tid tid' s s' r evs,
+      tid <> tid' ->
+      MailboxRestrictedAPI.step_allow op tid s ->
+      MailboxRestrictedAPI.step op' tid' s r s' evs ->
+      MailboxRestrictedAPI.step_allow op tid s'.
+  Proof.
+    intros.
+    destruct op; destruct op'; repeat step_inv; subst; eauto.
+    all: simpl in *; try congruence.
+  Qed.
+
+  Definition compile_ts (ts : @threads_state MailboxRestrictedAPI.opT) := ts.
+
+  Theorem compile_ts_no_atomics :
+    forall ts,
+      no_atomics_ts ts ->
+      no_atomics_ts (compile_ts ts).
+  Proof.
+    unfold compile_ts; eauto.
+  Qed.
+
+  Theorem absInitP :
+    forall s1 s2,
+      MailboxAPI.initP s1 ->
+      absR s1 s2 ->
+      MailboxRestrictedAPI.initP s2.
+  Proof.
+    eauto.
+  Qed.
+
+  Theorem compile_traces_match :
+    forall ts,
+      follows_protocol ts ->
+      no_atomics_ts ts ->
+      traces_match_abs absR
+        MailboxAPI.initP
+        MailboxAPI.step
+        MailboxRestrictedAPI.step (compile_ts ts) ts.
+  Proof.
+    unfold compile_ts, follows_protocol, absR.
+    unfold traces_match_abs; intros; subst.
+    clear H1.
+    specialize (H sm).
+    destruct H2.
+    induction H1; eauto.
+    specialize (H tid _ p) as Htid.
+    intuition idtac; repeat deex.
+
+    edestruct IHexec.
+      eapply follows_protocol_s_exec_tid_upd; eauto.
+      intros; eapply allowed_stable; eauto.
+      destruct result; eauto.
+
+    eexists; intuition idtac.
+    eapply ExecPrefixOne.
+      eauto.
+      eapply follows_protocol_preserves_exec_tid'; eauto.
+      eauto.
+    eauto.
+  Qed.
+
+End AtomicReaderRestricted'.
+
+
+Module AtomicReader :=
+  LinkWithRule MailboxAPI MailboxRestrictedAPI MailServerLockAbsAPI MailboxLockingRule
+               AtomicReaderRestricted' AtomicReaderRestricted.
