src/Mail2/MailServerLockAbsAPI.v
@@ -1,0 +1,56 @@
+Require Import POCS.
+Require Import String.
+Require Import MailServerAPI.
+
+
+Module MailServerLockAbsAPI <: Layer.
+
+  Import MailServerAPI.
+
+  Record state_rec := mk_state {
+    maildir : dir_contents;
+    locked : option nat;
+  }.
+
+  Definition opT := opT.
+  Definition State := state_rec.
+  Definition initP (s : State) := True.
+
+  Inductive xstep : forall T, opT T -> nat -> State -> T -> State -> list event -> Prop :=
+  | StepDeliver : forall m mbox fn tid lock,
+    ~ FMap.In fn mbox ->
+    xstep (Deliver m) tid
+      (mk_state mbox lock)
+      tt
+      (mk_state (FMap.add fn m mbox) lock)
+      nil
+  | StepPickup : forall mbox tid r lock,
+    FMap.is_permutation_kv r mbox ->
+    xstep Pickup tid
+      (mk_state mbox lock)
+      r
+      (mk_state mbox lock)
+      nil
+  | StepDelete : forall mbox tid id lock,
+    xstep (Delete id) tid
+      (mk_state mbox lock)
+      tt
+      (mk_state (FMap.remove id mbox) lock)
+      nil
+  | StepGetRequest : forall mbox tid r lock,
+    xstep GetRequest tid
+      (mk_state mbox lock)
+      r
+      (mk_state mbox lock)
+      (Event r :: nil)
+  | StepRespond : forall mbox tid T (v : T) lock,
+    xstep (Respond v) tid
+      (mk_state mbox lock)
+      tt
+      (mk_state mbox lock)
+      (Event v :: nil)
+  .
+
+  Definition step := xstep.
+
+End MailServerLockAbsAPI.
